Sync.

src/riot/asn1/ASN1.Spec.Value.BigInteger.fsti
@@ -1,11 +1,11 @@
 module ASN1.Spec.Value.BigInteger
 
 open ASN1.Spec.Base
-open LowParse.Spec.SeqBytes.Base
 
 open ASN1.Base
 open ASN1.Spec.Tag
 open ASN1.Spec.Length
+open ASN1.Spec.Bytes32
 open LowParse.Spec.DER
 
 open FStar.Integers
@@ -13,15 +13,21 @@ open FStar.Integers
 module U32 = FStar.UInt32
 module B32 = FStar.Bytes
 
+(*
+
+  encoded -----parse------>  decoded
+   bytes  <---serialize--- octet string
+*)
+
 unfold
 let big_integer_as_octet_string_t
 = x: datatype_of_asn1_type OCTET_STRING
-  { let (.[]) = B32.index in
-    v (dfst x) > 0 /\                      // no nil
+  { let (.[]) = B32.get in
+      v (dfst x) > 0 /\                    // no nil
     ( if (v (dfst x) > 1) then
-      ( (dsnd x).[0] =!= 0x00uy )  // no leading zero byte if length > 1
+      ( (dsnd x).[0ul] =!= 0x00uy )        // no leading zero byte if length > 1
       else ( True ) ) /\
-    ( if ((dsnd x).[0] >= 0x80uy) then   // leave one space for leading zero byte
+    ( if ((dsnd x).[0ul] >= 0x80uy) then   // leave one space for leading zero byte
       ( v (dfst x) <= asn1_length_max - 7 )
       else ( True ) ) }
 
@@ -47,74 +53,105 @@ let asn1_TLV_int32_of_big_integer
 
 unfold
 let valid_big_integer_as_octet_string_prop
-  (l: asn1_value_length_of_big_integer)
+  (len: asn1_value_int32_of_big_integer)
   (x: big_integer_as_octet_string_t)
 : Type0
-= v (dfst x) > 0 /\
-  ( let (.[]) = B32.index in
-    if l = 1 then
-    ( v (dfst x) == l /\ (dsnd x).[0] < 0x80uy )
-    else if ((dsnd x).[0] >= 0x80uy) then
-    ( v (dfst x) == l - 1 )
+= let (.[]) = B32.get in
+  v (dfst x) > 0 /\
+  ( if v len = 1 then
+    ( v (dfst x) == v len /\ (dsnd x).[0ul] < 0x80uy )
+    else if ((dsnd x).[0ul] >= 0x80uy) then
+    ( v (dfst x) == v len - 1 )
     else
-    ( v (dfst x) == l /\ (dsnd x).[0] > 0x00uy ) )
+    ( v (dfst x) == v len /\ (dsnd x).[0ul] > 0x00uy ) )
 
 (* ZT: Exposing them because one lemma needs `synth_..._inverse`. *)
-val filter_big_integer_as_octet_string
-  (l: asn1_value_length_of_big_integer)
-  (s: lbytes l)
+let filter_big_integer_as_octet_string
+  (len: asn1_value_int32_of_big_integer)
+  (s32: B32.lbytes32 len)
 : GTot bool
+= let (.[]) = B32.get in
+  v len > 0 &&
+  ( if (v len = 1) then
+    ( s32.[0ul] < 0x80uy )
+    else if (s32.[0ul] = 0x00uy) then
+    ( s32.[1ul] >= 0x80uy )
+    else
+    ( s32.[0ul] < 0x80uy ) )
 
-val synth_big_integer_as_octet_string
-  (l: asn1_value_length_of_big_integer)
-  (s: parse_filter_refine (filter_big_integer_as_octet_string l))
-: GTot (value: big_integer_as_octet_string_t
-               { valid_big_integer_as_octet_string_prop l value })
+let synth_big_integer_as_octet_string
+  (len: asn1_value_int32_of_big_integer)
+  (s32: parse_filter_refine (filter_big_integer_as_octet_string len))
+: Tot (value: big_integer_as_octet_string_t
+               { valid_big_integer_as_octet_string_prop len value })
+= let (.[]) = B32.get in
+  if (v len = 1) then
+  ( (|1ul, s32|) )
+  else if (s32.[0ul] = 0x00uy) then
+  ( (|len - 1ul, B32.slice s32 1ul len|) )
+  else
+  ( (|len, s32|) )
 
 val lemma_synth_big_integer_as_octet_string_injective
-  (l: asn1_value_length_of_big_integer)
+  (len: asn1_value_int32_of_big_integer)
 : Lemma (
-  synth_injective (synth_big_integer_as_octet_string l)
+  synth_injective (synth_big_integer_as_octet_string len)
 )
 
-val synth_big_integer_as_octet_string_inverse
-  (l: asn1_value_length_of_big_integer)
-  (value: big_integer_as_octet_string_t {valid_big_integer_as_octet_string_prop l value})
-: GTot (s32: parse_filter_refine (filter_big_integer_as_octet_string l)
-            { value == synth_big_integer_as_octet_string l s32 })
+let synth_big_integer_as_octet_string_inverse
+  (len: asn1_value_int32_of_big_integer)
+  (value: big_integer_as_octet_string_t {valid_big_integer_as_octet_string_prop len value})
+: Tot (s32: parse_filter_refine (filter_big_integer_as_octet_string len)
+            { value == synth_big_integer_as_octet_string len s32 })
+= let (.[]) = B32.get in
+  if len = 1ul then
+  ( dsnd value )
+  else if (dsnd value).[0ul] >= 0x80uy then
+  ( let s32 = B32.create 1ul 0x00uy `B32.append` dsnd value in
+    B32.extensionality (dsnd value) (B32.slice s32 1ul len);
+    assert (B32.reveal s32 == B32.reveal (B32.create 1ul 0x00uy) `Seq.append` B32.reveal (dsnd value));
+    assert (s32.[0ul] = B32.reveal s32 `Seq.index` 0);
+    assert (B32.reveal s32 `Seq.index` 0 == B32.create 1ul 0x00uy `B32.get` 0ul);
+    assert (B32.create 1ul 0x00uy `B32.get` 0ul == 0x00uy);
+    assert (s32.[0ul] == 0x00uy);
+    s32 )
+  else
+  ( dsnd value )
 
-let parse_big_integer_as_octet_string_kind (l: asn1_value_length_of_big_integer) = constant_size_parser_kind l
+let parse_big_integer_as_octet_string_kind (len: asn1_value_int32_of_big_integer) = constant_size_parser_kind (v len)
 
 noextract
 val parse_big_integer_as_octet_string
-  (l: asn1_value_length_of_big_integer)
-: parser (parse_big_integer_as_octet_string_kind l) (x: big_integer_as_octet_string_t {valid_big_integer_as_octet_string_prop l x})
+  (len: asn1_value_int32_of_big_integer)
+: parser
+    (parse_big_integer_as_octet_string_kind len)
+    (x: big_integer_as_octet_string_t {valid_big_integer_as_octet_string_prop len x})
 
 noextract
 val serialize_big_integer_as_octet_string
-  (l: asn1_value_length_of_big_integer)
-: serializer (parse_big_integer_as_octet_string l)
+  (len: asn1_value_int32_of_big_integer)
+: serializer (parse_big_integer_as_octet_string len)
 
 val lemma_serialize_big_integer_as_octet_string_unfold
-  (l: asn1_value_length_of_big_integer)
-  (value: get_parser_type (parse_big_integer_as_octet_string l))
+  (len: asn1_value_int32_of_big_integer)
+  (value: get_parser_type (parse_big_integer_as_octet_string len))
 : Lemma (
-  serialize (serialize_big_integer_as_octet_string l) value ==
-  serialize (serialize_seq_flbytes l) (synth_big_integer_as_octet_string_inverse l value))
+  serialize (serialize_big_integer_as_octet_string len) value ==
+  serialize (serialize_flbytes32 len) (synth_big_integer_as_octet_string_inverse len value))
 
 val lemma_serialize_big_integer_as_octet_string_size
-  (l: asn1_value_length_of_big_integer)
-  (value: get_parser_type (parse_big_integer_as_octet_string l))
+  (len: asn1_value_int32_of_big_integer)
+  (value: get_parser_type (parse_big_integer_as_octet_string len))
 : Lemma (
-  Seq.length (serialize (serialize_big_integer_as_octet_string l) value) == l)
+  Seq.length (serialize (serialize_big_integer_as_octet_string len) value) == v len)
 
 
 
 let parser_tag_of_big_integer_as_octet_string
   (x: big_integer_as_octet_string_t)
 : Tot (the_asn1_tag INTEGER & asn1_value_int32_of_big_integer)
-= let (.[]) = B32.index in
-  if ((dsnd x).[0] >= 0x80uy) then
+= let (.[]) = B32.get in
+  if ((dsnd x).[0ul] >= 0x80uy) then
   ( (INTEGER, dfst x + 1ul) )
   else
   ( (INTEGER, dfst x) )
@@ -164,7 +201,7 @@ val lemma_serialize_big_integer_as_octet_string_TLV_unfold
   `Seq.append`
   serialize (serialize_asn1_length_of_big_integer) (snd tg)
   `Seq.append`
-  serialize (serialize_big_integer_as_octet_string (v (snd tg))) value
+  serialize (serialize_big_integer_as_octet_string (snd tg)) value
 )
 
 let len_of_big_integer_as_octet_string_TLV
@@ -179,3 +216,17 @@ val lemma_serialize_big_integer_as_octet_string_TLV_size
   Seq.length (serialize serialize_big_integer_as_octet_string_TLV value) ==
   v (len_of_big_integer_as_octet_string_TLV value)
 )
+
+let asn1_get_octet_string
+  (len: asn1_value_int32_of_type OCTET_STRING)
+  (s32: B32.lbytes32 len)
+: Tot (datatype_of_asn1_type OCTET_STRING)
+= (|len, s32|)
+
+(* Given a big integer in bytes, returns the _encoded_ octet string. *)
+let asn1_get_big_integer_as_octet_string
+  (len: asn1_value_int32_of_big_integer)
+  (s32: B32.lbytes32 len
+        { filter_big_integer_as_octet_string len s32 })
+: Tot (big_integer_as_octet_string_t)
+= synth_big_integer_as_octet_string len s32
