src/riot/asn1/ASN1.Low.Value.BigInteger.fsti
@@ -4,6 +4,7 @@ open ASN1.Base
 open ASN1.Low.Base
 open ASN1.Low.Tag
 open ASN1.Low.Length
+open ASN1.Low.Bytes32
 open ASN1.Low.Value.OCTET_STRING
 open ASN1.Spec.Value.BigInteger
 module HS = FStar.HyperStack
@@ -25,7 +26,7 @@ let serialize32_asn1_length_of_big_integer_backwards
 inline_for_extraction
 val serialize32_big_integer_as_octet_string_backwards
   (len: asn1_value_int32_of_big_integer)
-: Tot (serializer32_backwards (serialize_big_integer_as_octet_string (v len)))
+: Tot (serializer32_backwards (serialize_big_integer_as_octet_string len))
 
 noextract inline_for_extraction
 let parser_tag_of_big_integer_as_octet_string_impl
