src/riot/x509/X509.BasicFields.SerialNumber.fsti
@@ -29,16 +29,23 @@ module B32 = FStar.Bytes
 
 (* NOTE: 1. `big_integer_as_octet_string_t` is the UN-ENCODED PLAIN integer represented as octets;
          2. the 20 octets restriction is on this plain serialNumber value. *)
-let filter_x509_serialNumber
-  (x: big_integer_as_octet_string_t)
+
+let filter_x509_serialNumber_from_s32
+  (len: asn1_value_int32_of_big_integer)
+  (s32: B32.lbytes32 len)
 : GTot bool
-= let (|len, s32|) = x in
+=
 (* Conforming RFC 5280 -- serialNumber __value__ should not longer then 20 octets *)
   len <= 20ul &&
 (* Non-Negative -- the first bit is zero *)
   B32.index s32 0 < 0x80uy &&
 (* Non-Zero -- when length is 1, the only octet is not 0 *)
  (len > 1ul || B32.index s32 0 > 0x00uy)
+
+let filter_x509_serialNumber
+  (x: big_integer_as_octet_string_t)
+: GTot bool
+= filter_x509_serialNumber_from_s32 (dfst x) (dsnd x)
 
 let x509_serialNumber_t
 = parse_filter_refine filter_x509_serialNumber
@@ -63,7 +70,7 @@ val lemma_serialize_x509_serialNumber_unfold
   `Seq.append`
  (serialize_asn1_length_of_big_integer `serialize` (snd tg))
   `Seq.append`
- (serialize_big_integer_as_octet_string (v (snd tg)) `serialize` x)
+ (serialize_big_integer_as_octet_string (snd tg) `serialize` x)
 )
 
 noextract unfold [@@ "opaque_to_smt"]
@@ -87,3 +94,10 @@ let len_of_x509_serialNumber
 
 val serialize32_x509_serialNumber_backwards
 : serializer32_backwards serialize_x509_serialNumber
+
+// let x509_get_serialNumber
+//   (len: asn1_value_int32_of_big_integer)
+//   (s32: B32.lbytes32 len
+//         { filter_x509_serialNumber_from_s32 len s32 })
+// = asn1_get_big_integer_as_octet_string len s32
+
