src/riot/x509/X509.ExtFields.KeyUsage.fst
@@ -41,14 +41,14 @@ let x509_KU_CRL_SIGN          = 0x02l    (* bit 6 *)
 let x509_KU_ENCIPHER_ONLY     = 0x01l    (* bit 7 *)
 let x509_KU_DECIPHER_ONLY     = 0x8000l  (* bit 8 *)
 
-(* FIXME: Can we normalize bitwise operators? *)
-let lemma_key_usage_close_under_or ku1 ku2
-= admit()
+// (* FIXME: Can we normalize bitwise operators? *)
+// let lemma_key_usage_close_under_or ku1 ku2
+// = admit()
 
-let op_ku_with ku1 ku2
-= [@inline_let]let ku: int_32 = ku1 |^ ku2 in
-  lemma_key_usage_close_under_or ku1 ku2;
-  ku
+// let op_ku_with ku1 ku2
+// = [@inline_let]let ku: int_32 = ku1 |^ ku2 in
+//   lemma_key_usage_close_under_or ku1 ku2;
+//   ku
 
 let _filter_x509_key_usage_payload
   (bs: datatype_of_asn1_type BIT_STRING)
